---
author: James  Watmough
date: "`r Sys.Date()`"
---

{{< include texmacros.qmd >}}

# The Derivative {#sec-differentiation}

## Secant and Tangent Lines {#sec-diff-def}

## Derivatives of Our Core Functions {#sec-diff-rules-I}

There are a few properties of derivatives that will save us from having to compute limits every time we need to differentiate a function.  These should be memorized over the next few weeks.

|   |   |   |
|:-------------|:--------------------------------------------------------------------------:|:------------------|
|Constant Rule: | $\frac{d}{dx} \text{constant} = 0$ |   |
|Power Rule:    | $\frac{d}{dx} x^n = nx^{n-1}$  | for any real number $n$  |
|Scaling Rule:  | $\frac{d}{dx} cf(x) = cf'(x)$  | for any constant $c$  |
|Sum Rule:      | $\frac{d}{dx} \left(f(x)+g(x)\right) = f'(x)+g'(x)$  |    |
|Product Rule:  | $\frac{d}{dx} \left(f(x)g(x)\right) = f'(x)g(x)+f(x)g'(x)$  |    |
|Quotient Rule: | $\frac{d}{dx} \dfrac{f(x)}{g(x)} = \dfrac{f'(x)g(x)-f(x)g'(x)}{(g(x))^2}$  |    |

The first three rules let us easily differentiate polynomials.  The product and quotient rules help differentiate more complex functions.

In addition, you should memorize the derivatives of our core set of transcendental functions

|                |                |                   |
|:---------------|:--------------:|:------------------|
| Exponential:   | $\frac{d}{dx} a^x = a^x \log(a)$   | $a>0$ | 
| Logarithmic:   | $\frac{d}{dx} \log_a x = \frac{1}{x \log(a)}$   | $x>0$ | 
| Trigonometric: | $\frac{d}{dx} \sin x = \cos x$   | | 
|                | $\frac{d}{dx} \cos x =-\sin x$   | | 
|                | $\frac{d}{dx} \tan x = (\sec x)^2$   | | 

Proofs of these rules are available on request.  I will give some hints during lectures but the details will be left to supplementary material.

## The Product and Quotient Rules {#sec-diff-rules-2}

One way to help remember the product rule is to consider a rectangle with sides of length $f$ and $g$.  The area of this rectangle is the product $fg$.  If we change the length of the second side by a small amount, say from $g$ to $g+dg$, then the area changes from $fg$ to $f(g+dg)$.  That's a change of $f\,dg$.  If we change the length of the first side, the change in the area is $df\, g$.  Adding these two together gives us something that looks like the product rule:  $df\,g + f\,dg$.  The details of how these calculations look using limits are given in the text.

::: {#exm-diff-product-1}

Differentiate $x \log x$

:::

::: {.callout-tip collapse=true title="solution"}

\begin{align*}
\frac{d}{dx} \left( x \log x \right) &= \log(x) + x\frac{d}{dx} \log x \\
                                     &= \log(x) + x\frac{1}{x} \\
                                     &= 1 + \log(x) \\
\end{align*}

:::

::: {#exm-diff-product-2}

Differentiate $x e^x\sin x$

:::

::: {.callout-tip collapse=true title="solution"}

We apply the product rule twice.  The order doesn't matter.

\begin{align*}
\frac{d}{dx} \left( x e^x\sin x \right) 
&= \left(\frac{d}{dx} xe^x\right)\sin x  + xe^x\frac{d}{dx}\sin x \\
&= \left(e^x  + xe^x\right)\sin x + xe^x\cos x \\
&= \left(1+x)\right)e^x\sin x + xe^x\cos x
\end{align*}

:::

The origin of the quotient rule doesn't have as simple a geometric motivation as the product rule, but it can be easily derived from the product rule.
First, start by naming the ratio $F$
$$F(x) = \frac{f(x)}{g(x)}$$
Then rewrite this as a product
$$F(x)g(x) = f(x)$$
Now differentiate both sides of the equality.
$$F'(x)g(x) + F(x)g'(x) = f'(x)$$
Replace $F$ by the ratio
$$F'(x)g(x) + \frac{f(x)}{g(x)}g'(x) = f'(x)$$
and isolate $F'$ on the left side
$$F'(x) = \frac{f'(x)}{g(x)} - \frac{f(x)g'(x)}{(g(x))^2}$$

::: {#exm-diff-quotient-1}

Find the derivative of $\tan x$

:::

::: {.callout-tip collapse=true title="solution"}

\begin{align*}
\frac{d}{dx} \tan x 
&= \frac{d}{dx} \frac{\sin x}{\cos x} \\
&= \frac{ \left(\frac{d}{dx} \sin x \right) \cos x - \sin x \frac{d}{dx} \cos x  }{(\cos x)^2} \\
&= \frac{ \cos x \cos x - (\sin x)(-\sin x)  }{(\cos x)^2} \\
&= \frac{ (\cos x)^2  + (\sin x)^2  }{(\cos x)^2} \\
&= \frac{1}{(\cos x)^2} \\
&= (\sec x)^2 
\end{align*}

We can also write this as $1 + (\tan x)^2$

:::

::: {#exm-diff-quotient-1}

Where does $x\mapsto \dfrac{3x}{4 + x^2}$ have a horizontal tangent?

:::

::: {.callout-tip collapse=true title="solution"}

We're being asked to find where the derivative of $\dfrac{3x}{4 + x^2}$ is zero.  Use the quotient rule to find the derivative.

\begin{align*}
\frac{d}{dx} \dfrac{3x}{4 + x^2} 
&= \frac{ (3)(4+x^2) - (3x)(0+2x) }{(4+x^2)} \\
&= \frac{ 12 - 3x^2 }{(4+x^2)} 
\end{align*}

The denominator is always positive (no vertical tangent lines) and the numerator is zero when $x$ is either 2 or -2.

:::
